cedar-lean/Cedar/Thm/SymCC/Env/Soundness.lean
@@ -30,21 +30,37 @@ open Cedar.Thm
 open Cedar.Spec
 open Cedar.SymCC
 open Cedar.Validation
+open Cedar.Data
 
-/--
-`Value.symbolize?` is total on well-typed values,
-and the resulting term is a well-formed literal
--/
-theorem value_symbolize?_same
-  {Γ : TypeEnv} {v : Value} {ty : CedarType}
-  (hwf : Γ.WellFormed)
+theorem filterMap_mapM_combine
+  {l₁ : List α} {l₂ : List β}
+  {f : α → Option β}
+  {g : β → Option γ}
+  (h : l₁.mapM f = .some l₂) :
+  -- (hh : ∀ x ∈ l₁, ∃ y, (f x).bind g = .some y) :
+  l₂.filterMap g = l₁.filterMap (λ x => (f x).bind g)
+:= by
+  sorry
+
+theorem filterMap_partial_inverse
+  {l : List α}
+  {f : α → Option α}
+  (h : ∀ x ∈ l, f x = .some x) :
+  l.filterMap f = l
+:= sorry
+
+theorem value?_symbolize?_id
+  {Γ : TypeEnv} {entities : Entities}
+  {v : Value} {ty : CedarType}
+  (hwf_Γ : Γ.WellFormed)
   (hwf_ty : ty.WellFormed Γ)
-  (hwt : InstanceOfType Γ v ty) :
+  (hwf_v : v.WellFormed entities)
+  (hwt_v : InstanceOfType Γ v ty) :
   ∃ t,
     v.symbolize? ty = .some t ∧
-    v ∼ t
+    t.value? = .some v
 := by
-  cases hwt with
+  cases hwt_v with
   | instance_of_bool
   | instance_of_string
   | instance_of_entity
@@ -55,14 +71,518 @@ theorem value_symbolize?_same
       Same.same, SameValues,
       Term.value?, TermPrim.value?, BitVec.int64?,
     ]
-  | instance_of_set s sty hwt =>
-    simp [Value.symbolize?]
-    sorry
-  | instance_of_record rec =>
-    sorry
+  | instance_of_set elems elem_ty hwt_elem =>
+    cases hwf_ty with | set_wf hwf_elem_ty =>
+    cases hwf_v with | set_wf hwf_elem hwf_set_elems =>
+    simp only [Value.symbolize?]
+    -- Some facts about calling `symbolize?` on the elements
+    have ⟨sym_elems, hsym_elems, hval_sym_elems_id⟩ :
+      ∃ sym_elems,
+        elems.toList.mapM (λ x => x.symbolize? elem_ty)
+        = .some sym_elems ∧
+        ∀ sym_elem ∈ sym_elems,
+          ∃ elem ∈ elems, sym_elem.value? = .some elem
+    := by
+      have (elem : Value) (hmem_elem : elem ∈ elems.toList) :
+        ∃ sym_elem,
+          elem.symbolize? elem_ty = .some sym_elem
+      := by
+        have ⟨sym_elem, hsym_elem, _⟩ := value?_symbolize?_id hwf_Γ hwf_elem_ty (hwf_elem elem hmem_elem) (hwt_elem elem hmem_elem)
+        exists sym_elem
+      have ⟨sym_elems, hsym_elems⟩ := List.all_some_implies_mapM_some this
+      simp only [hsym_elems, Option.some.injEq, exists_eq_left']
+      intros sym_elem hmem_sym_elem
+      have ⟨elem, hmem_elem, hsym_elem⟩ := List.mapM_some_implies_all_from_some hsym_elems sym_elem hmem_sym_elem
+      simp only [Set.toList] at hmem_elem
+      exists elem
+      simp only [(Set.in_list_iff_in_set _ _).mp hmem_elem, true_and]
+      have ⟨sym_elem', hsym_elem', hval_sym_elem'⟩ := value?_symbolize?_id hwf_Γ hwf_elem_ty (hwf_elem elem hmem_elem) (hwt_elem elem hmem_elem)
+      have : sym_elem' = sym_elem := by
+        simp only [hsym_elem', Option.some.injEq] at hsym_elem
+        exact hsym_elem
+      simp only [this] at hval_sym_elem'
+      exact hval_sym_elem'
+    -- Some facts about calling `value?` on the symbolized elements
+    have ⟨val_sym_elems, hval_sym_elems, hval_sym_elem_inv⟩ :
+      ∃ val_sym_elems,
+        (Set.make sym_elems).1.mapM Term.value?
+        = .some val_sym_elems ∧
+        ∀ val_sym_elem ∈ val_sym_elems,
+          ∃ sym_elem ∈ sym_elems, val_sym_elem = sym_elem.value?
+    := by
+      have (sym_elem : Term) (hmem_sym_elem : sym_elem ∈ (Set.make sym_elems)) :
+        ∃ val_sym_elem,
+          sym_elem.value? = .some val_sym_elem
+      := by
+        have hmem_sym_elem := (Set.make_mem _ _).mpr hmem_sym_elem
+        have ⟨elem, hmem_elem, hsym_elem⟩ := List.mapM_some_implies_all_from_some hsym_elems sym_elem hmem_sym_elem
+        exists elem
+        have ⟨sym_elem', hsym_elem', hval_sym_elem'⟩ := value?_symbolize?_id hwf_Γ hwf_elem_ty (hwf_elem elem hmem_elem) (hwt_elem elem hmem_elem)
+        have : sym_elem' = sym_elem := by
+          simp only [hsym_elem', Option.some.injEq] at hsym_elem
+          exact hsym_elem
+        simp only [this] at hval_sym_elem'
+        exact hval_sym_elem'
+      have ⟨val_sym_elems, hval_sym_elems⟩ := List.all_some_implies_mapM_some this
+      simp only [hval_sym_elems, Option.some.injEq, exists_eq_left']
+      intros val_sym_elem hmem_val_sym_elem
+      have ⟨sym_elem', hmem_sym_elem', hval_sym_elem'⟩ := List.mapM_some_implies_all_from_some hval_sym_elems val_sym_elem hmem_val_sym_elem
+      exists sym_elem'
+      simp only [(Set.make_mem _ _).mpr hmem_sym_elem', true_and]
+      simp [hval_sym_elem']
+    -- Simplify the goal with the facts above
+    simp only [
+      List.mapM₁_eq_mapM (λ x => x.symbolize? elem_ty) elems.toList,
+      hsym_elems,
+    ]
+    simp only [Option.bind_some_fun, Option.some.injEq, exists_eq_left']
+    unfold Term.value?
+    simp only [hval_sym_elems, List.mapM₁_eq_mapM _ _]
+    simp only [Option.bind_some_fun, Option.some.injEq, Value.set.injEq]
+    -- Prove that the sets of values before and after `value? ∘ symbolize?` are equal
+    apply (Set.subset_iff_eq (Set.make_wf _) hwf_set_elems).mp
+    constructor
+    · apply Set.subset_def.mpr
+      intros val_sym_elem hmem_val_sym_elem
+      replace hmem_val_sym_elem := (Set.make_mem _ _).mpr hmem_val_sym_elem
+      have ⟨sym_elem, hmem_sym_elem, hval_sym_elem⟩ := hval_sym_elem_inv val_sym_elem hmem_val_sym_elem
+      have ⟨elem', hmem_elem', hval_sym_elem'⟩ := hval_sym_elems_id sym_elem hmem_sym_elem
+      simp only [hval_sym_elem', Option.some.injEq] at hval_sym_elem
+      simp only [hval_sym_elem, hmem_elem']
+    · apply Set.subset_def.mpr
+      intros elem hmem_elem
+      have ⟨sym_elem, hmem_sym_elem, hsym_elem⟩ := List.mapM_some_implies_all_some hsym_elems elem hmem_elem
+      replace hmem_sym_elem := (Set.make_mem _ _).mp hmem_sym_elem
+      have ⟨val_sym_elem, hmem_val_sym_elem, hval_sym_elem⟩ := List.mapM_some_implies_all_some hval_sym_elems sym_elem hmem_sym_elem
+      have ⟨sym_elem', hsym_elem', hval_sym_elem'⟩ := value?_symbolize?_id hwf_Γ hwf_elem_ty (hwf_elem elem hmem_elem) (hwt_elem elem hmem_elem)
+      have : sym_elem' = sym_elem := by
+        simp only [hsym_elem', Option.some.injEq] at hsym_elem
+        exact hsym_elem
+      have : val_sym_elem = elem := by
+        simp only [this] at hval_sym_elem'
+        simp only [hval_sym_elem', Option.some.injEq] at hval_sym_elem
+        simp [hval_sym_elem]
+      simp only [this] at hmem_val_sym_elem
+      exact (Set.make_mem _ _).mp hmem_val_sym_elem
+  | _ => sorry
+
+-- /--
+-- `Value.symbolize?` is a partial inverse of `Term.value?`.
+-- -/
+-- theorem value?_symbolize?_id
+--   {Γ : TypeEnv} {entities : Entities} {v : Value} {t : Term} {ty : CedarType}
+--   (hwf : Γ.WellFormed)
+--   (hwf_ty : ty.WellFormed Γ)
+--   (hwf_v : v.WellFormed entities)
+--   (hwt : InstanceOfType Γ v ty)
+--   (hok : v.symbolize? ty = .some t) :
+--   t.value? = .some v
+-- := by
+--   cases hwt with
+--   | instance_of_bool
+--   | instance_of_string
+--   | instance_of_entity
+--   | instance_of_ext
+--   | instance_of_int =>
+--     simp only [Value.symbolize?, Prim.symbolize, Option.some.injEq] at hok
+--     simp [←hok, Term.value?, TermPrim.value?, BitVec.int64?]
+--   | instance_of_set s sty hwt =>
+--     cases hwf_ty with | set_wf hwf_sty =>
+--     cases hwf_v with | set_wf hwf_v hwf_s =>
+--     simp only [
+--       Value.symbolize?, Option.bind_eq_bind,
+--       bind, Option.bind,
+--     ] at hok
+--     split at hok
+--     contradiction
+--     rename_i ts hts
+--     simp only [List.mapM₁_eq_mapM (λ v => v.symbolize? sty) s.toList] at hts
+--     simp only [Option.some.injEq] at hok
+--     simp only [←hok]
+--     -- `symbolize?` on elements should succeed
+--     have ⟨vs, hvs⟩ :
+--       ∃ vs,
+--         (Set.make ts).1.mapM (λ t => t.value?) = .some vs
+--     := by
+--       apply List.all_some_implies_mapM_some
+--       intros t hmem_t
+--       have := (Set.make_mem _ _).mpr hmem_t
+--       have hts := List.mapM_some_implies_all_from_some hts
+--       have ⟨x, hmem_x, hsym_x⟩ := hts t this
+--       have hwt_x := hwt x hmem_x
+--       have hsame_y := value?_symbolize?_id hwf hwf_sty (hwf_v x hmem_x) hwt_x hsym_x
+--       exists x
+--     unfold Term.value?
+--     simp only [
+--       List.mapM₁_eq_mapM ?_ (Set.make ts).1,
+--       hvs,
+--       Option.bind_some_fun, Option.some.injEq,
+--       Value.set.injEq,
+--     ]
+--     -- Prove that the sets of values before and after `value? ∘ symbolize?` are equal
+--     apply (Set.subset_iff_eq (Set.make_wf _) hwf_s).mp
+--     constructor
+--     · apply Set.subset_def.mpr
+--       intros new_v hmem_new_v
+--       have hmem_new_v := (Set.make_mem _ _).mpr hmem_new_v
+--       have ⟨x, hmem_x, hx_value?⟩ := List.mapM_some_implies_all_from_some hvs new_v hmem_new_v
+--       have hmem_x := (Set.make_mem _ _).mpr hmem_x
+--       have ⟨old_v, hmem_old_v, hold_v_symbolize?⟩ := List.mapM_some_implies_all_from_some hts x hmem_x
+--       have := value?_symbolize?_id hwf hwf_sty (hwf_v old_v hmem_old_v) (hwt old_v hmem_old_v) hold_v_symbolize?
+--       simp only [this, Option.some.injEq] at hx_value?
+--       simp only [hx_value?] at hmem_old_v
+--       exact hmem_old_v
+--     · apply Set.subset_def.mpr
+--       intros old_v hmem_old_v
+--       have ⟨t, hmem_t, hv_symbolize?⟩ := List.mapM_some_implies_all_some hts old_v hmem_old_v
+--       have ⟨new_v, hmem_new_v, hnew_v_symbolize?⟩ := List.mapM_some_implies_all_some hvs t ((Set.make_mem _ _).mp hmem_t)
+--       have := value?_symbolize?_id hwf hwf_sty (hwf_v old_v hmem_old_v) (hwt old_v hmem_old_v) hv_symbolize?
+--       simp only [this, Option.some.injEq] at hnew_v_symbolize?
+--       simp only [←hnew_v_symbolize?] at hmem_new_v
+--       exact (Set.make_mem _ _).mp hmem_new_v
+--   | instance_of_record rec rty h₁ h₂ h₃ =>
+--     cases hwf_ty with | record_wf hwf_rty_map hwf_rty =>
+--     cases hwf_v with | record_wf hwf_v hwf_rec_map =>
+--     simp only [
+--       Value.symbolize?,
+--       Option.bind_eq_bind,
+--       bind, Option.bind,
+--     ] at hok
+--     -- have := List.mapM₂_eq_mapM (λ x =>
+--     --     (Map.find? rty x.fst).bind fun __do_lift =>
+--     --       match __do_lift with
+--     --       | Qualified.optional ty => (x.snd.symbolize? ty).bind fun __do_lift => some (x.fst, __do_lift.some)
+--     --       | Qualified.required ty => (x.snd.symbolize? ty).bind fun __do_lift => some (x.fst, __do_lift))
+--     --     rec.toList
+--     -- simp [Subtype.val] at this
+--     -- -- have := Eq.trans (Eq.symm hok) this
+--     -- have := List.mapM₂_eq_mapM (λ x => do
+--     --       match ← Map.find? rty x.fst with
+--     --       | .optional ty => .some (x.fst, Term.some (← x.snd.symbolize? ty))
+--     --       | .required ty => .some (x.fst, ← x.snd.symbolize? ty))
+--     --     rec.toList
+--     -- simp [this] at hok
+--     -- have [SizeOf Attr] [SizeOf Term] [i : SizeOf Value] :
+--     --   (rec.toList.mapM₂ fun (x : {x : Attr × Value // i.sizeOf x.snd < 1 + sizeOf rec.toList}) =>
+--     --     (Map.find? rty x.1.fst).bind fun __do_lift =>
+--     --       match __do_lift with
+--     --       | Qualified.optional ty => (x.1.snd.symbolize? ty).bind fun __do_lift => some (x.1.fst, __do_lift.some)
+--     --       | Qualified.required ty => (x.1.snd.symbolize? ty).bind fun __do_lift => some (x.1.fst, __do_lift)) =
+--     --   (rec.toList.mapM fun x =>
+--     --     (Map.find? rty x.fst).bind fun __do_lift =>
+--     --       match __do_lift with
+--     --       | Qualified.optional ty => (x.snd.symbolize? ty).bind fun __do_lift => some (x.fst, __do_lift.some)
+--     --       | Qualified.required ty => (x.snd.symbolize? ty).bind fun __do_lift => some (x.fst, __do_lift))
+--     -- :=
+--     --   List.mapM₂_eq_mapM
+--     --     (fun x =>
+--     --     (Map.find? rty x.fst).bind fun __do_lift =>
+--     --       match __do_lift with
+--     --       | Qualified.optional ty => (x.snd.symbolize? ty).bind fun __do_lift => some (x.fst, __do_lift.some)
+--     --       | Qualified.required ty => (x.snd.symbolize? ty).bind fun __do_lift => some (x.fst, __do_lift))
+--     --     rec.toList
+--     -- simp only [this] at hok
+--     split at hok
+--     contradiction
+--     simp only [Option.some.injEq] at hok
+--     rename_i ts hts
+--     simp only [←hok]
+--     have ⟨vs, hvs⟩ :
+--       ∃ vs,
+--         (Map.mk ts).1.mapM (λ (a, t) => Term.value?.attrValue? a t)
+--         = .some vs
+--     := by
+--       apply List.all_some_implies_mapM_some
+--       intros p hmem_p
+--       simp only
+--       unfold Term.value?.attrValue?
+--       have hts := List.mapM_some_implies_all_from_some hts
+--       have ⟨x, hmem_x, hsym_x⟩ := hts p hmem_p
+--       simp only [List.attach₂] at hmem_x
+--       have ⟨x', hmem_x', hxx'⟩ := List.mem_pmap.mp hmem_x
+--       split at hsym_x
+--       contradiction
+--       rename_i qty hfind_qty
+--       simp only at hsym_x
+--       -- Type of sym_x is well-formed
+--       have hxx' : x.1 = x' := by simp [←hxx']
+--       simp only [hxx'] at hfind_qty
+--       have hwf_qty := hwf_rty x'.fst qty hfind_qty
+--       have hrec_find := (Map.in_list_iff_find?_some hwf_rec_map).mp hmem_x'
+--       have hwf_x' := hwf_v x'.fst x'.snd hrec_find
+--       have hwt_x' := h₂ x'.fst x'.snd qty hrec_find hfind_qty
+--       cases hqty : qty with
+--       | optional ty =>
+--         simp only [hqty] at hsym_x
+--         split at hsym_x
+--         contradiction
+--         rename_i sym_x hsym_x_ok
+--         simp only [Option.some.injEq] at hsym_x
+--         simp [←hsym_x]
+--         have ⟨v, hv⟩ : ∃ v, sym_x.value? = .some v := by
+--           simp only [hqty] at hwf_qty
+--           cases hwf_qty with | optional_wf hwf_ty =>
+--           simp only [hxx'] at hsym_x_ok
+--           simp only [hqty] at hwt_x'
+--           have := value?_symbolize?_id hwf hwf_ty hwf_x' hwt_x' hsym_x_ok
+--           simp [this]
+--         simp [hv]
+--       | required ty =>
+--         simp only [hqty] at hsym_x
+--         split at hsym_x
+--         contradiction
+--         rename_i sym_x hsym_x_ok
+--         simp only [Option.some.injEq] at hsym_x
+--         simp [←hsym_x]
+--         have ⟨v, hv⟩ : ∃ v, sym_x.value? = .some v := by
+--           simp only [hqty] at hwf_qty
+--           cases hwf_qty with | required_wf hwf_ty =>
+--           simp only [hxx'] at hsym_x_ok
+--           simp only [hqty] at hwt_x'
+--           have := value?_symbolize?_id hwf hwf_ty hwf_x' hwt_x' hsym_x_ok
+--           simp [this]
+--         split
+--         · simp [Term.value?] at hv
+--         · simp [Term.value?] at hv
+--         simp [hv]
+--     unfold Term.value?
+--     simp only [
+--       hvs,
+--       List.mapM₂_eq_mapM
+--         (fun x => Term.value?.attrValue? x.fst x.snd)
+--         (Map.mk ts).1,
+--       Option.bind_some_fun, Option.some.injEq,
+--       Value.record.injEq,
+--     ]
+--     cases rec with | mk rec =>
+--     simp only [Map.mk.injEq]
+
+--     have hts :
+--       List.mapM
+--       (fun x =>
+--         match Map.find? rty x.fst, fun __do_lift =>
+--             match __do_lift with
+--             | Qualified.optional ty =>
+--               match x.snd.symbolize? ty, fun __do_lift => some (x.fst, __do_lift.some) with
+--               | none, x => none
+--               | some a, f => f a
+--             | Qualified.required ty =>
+--               match x.snd.symbolize? ty, fun __do_lift => some (x.fst, __do_lift) with
+--               | none, x => none
+--               | some a, f => f a with
+--           | none, x => none
+--           | some a, f => f a)
+--         (Map.mk rec).toList =
+--       some ts
+--     := by
+--       apply Eq.symm
+
+--       -- have := (List.mapM₂_eq_mapM (fun x =>
+--       --   match Map.find? rty x.fst, fun __do_lift =>
+--       --       match __do_lift with
+--       --       | Qualified.optional ty =>
+--       --         match x.snd.symbolize? ty, fun __do_lift => some (x.fst, Term.some __do_lift) with
+--       --         | none, x => none
+--       --         | some a, f => f a
+--       --       | Qualified.required ty =>
+--       --         match x.snd.symbolize? ty, fun __do_lift => some (x.fst, __do_lift) with
+--       --         | none, x => none
+--       --         | some a, f => f a with
+--       --     | none, x => none
+--       --     | some a, f => f a) (Map.mk rec).toList)
+--       -- have := List.mapM₂_eq_mapM (λ ⟨a, v⟩ => do
+--       --   match ← rty.find? a with
+--       --   | .optional ty => .some (a, Option.some (← v.symbolize? ty))
+--       --   | .required ty => .some (a, ← v.symbolize? ty)) (Map.mk rec).toList
+
+--       -- simp [this]
+
+--       -- apply Eq.trans (Eq.symm hts) this
+
+--       sorry
+
+--     rw [filterMap_mapM_combine hvs]
+--     rw [filterMap_mapM_combine hts]
+--     simp only [Map.toList, Map.kvs]
+--     apply filterMap_partial_inverse
+--     intros p hmem_p
+
+--     split
+--     · simp only [Option.bind_none, reduceCtorEq]
+--       rename_i hnot_find
+--       have hmem_p := (Map.in_list_iff_find?_some hwf_rec_map).mp hmem_p
+--       have := h₁ p.fst
+--       unfold Map.contains at this
+--       simp only [Option.isSome, hmem_p, forall_const] at this
+--       split at this
+--       · rename_i h
+--         simp [h] at hnot_find
+--       · contradiction
+--     rename_i qty hfind_qty
+--     simp only
+--     cases qty with
+--     | optional ty =>
+--       simp only
+--       split
+--       · rename_i hsym_p_nok
+--         have ⟨y, hmem_y, hyok⟩ := List.mapM_some_implies_all_some hts p hmem_p
+--         split at hyok
+--         contradiction
+--         simp only at hyok
+--         rename_i hrty_find
+--         simp only [hfind_qty, Option.some.injEq] at hrty_find
+--         simp only [←hrty_find] at hyok
+--         simp only [hsym_p_nok] at hyok
+--         contradiction
+--       · rename_i hsym_p hsym_p_ok
+--         simp only [Option.bind_some, Term.value?.attrValue?]
+
+--         sorry
+--     | required ty =>
+--       sorry
+
+--     -- have ⟨y, hmem_y, hyok⟩ := List.mapM_some_implies_all_some hts p hmem_p
+--     -- simp only [hyok, Option.bind_some]
+--     -- have ⟨z, hmem_z, hzok⟩ := List.mapM_some_implies_all_some hvs y hmem_y
+--     -- simp only [hzok, Option.bind_some]
+
+--     -- have : ∀ v ∈ vs, ∃ v', v.2 = .some v' := by
+--     --   sorry
+
+--     -- have ⟨z', hz'⟩ := this z hmem_z
+--     -- simp [hz']
+--     -- all_goals sorry
+
+--     -- apply List.filterMap_unattach
+
+--     -- apply filterMap_always_some_eq
+--     -- apply List.forall₂_iff_map_eq
+
+--     -- simp [
+--     --   List.mapM₂_eq_mapM (fun x =>
+--     --   match Map.find? rty x.fst, fun __do_lift =>
+--     --     match __do_lift with
+--     --     | Qualified.optional ty =>
+--     --       match x.snd.symbolize? ty, fun __do_lift => some (x.fst, Option.some __do_lift) with
+--     --       | none, x => none
+--     --       | some a, f => f a
+--     --     | Qualified.required ty =>
+--     --       match x.snd.symbolize? ty, fun __do_lift => some (x.fst, __do_lift) with
+--     --       | none, x => none
+--     --       | some a, f => f a with
+--     --   | none, x => none
+--     --   | some a, f => f a) rec.toList
+--     -- ] at hts
+
+--     -- have := List.mapM₂_eq_mapM (fun x =>
+--     --     (Map.find? rty x.fst).bind fun __do_lift =>
+--     --       match __do_lift with
+--     --       | Qualified.optional ty => (x.snd.symbolize? ty).bind fun __do_lift => some (x.fst, __do_lift.some)
+--     --       | Qualified.required ty => (x.snd.symbolize? ty).bind fun __do_lift => some (x.fst, __do_lift)) rec.toList
+
+--     -- simp [this] at hts
+--     -- have ⟨ts, hts⟩ :
+--     --   ∃ ts,
+--     --   (rec.toList.mapM₂ fun x =>
+--     --     (Map.find? rty x.1.fst).bind fun __do_lift =>
+--     --       match __do_lift with
+--     --       | Qualified.optional ty => (x.1.snd.symbolize? ty).bind fun __do_lift => some (x.1.fst, __do_lift.some)
+--     --       | Qualified.required ty => (x.1.snd.symbolize? ty).bind fun __do_lift => some (x.1.fst, __do_lift)) = .some ts
+--     -- := by
+--     --   sorry
+--     -- rw [hts] at hok
+
+--     -- sorry
+
+-- /--
+-- `Value.symbolize?` is total on well-typed values,
+-- and the resulting term is a well-formed literal
+
+-- TODO: might need an additional assumption `v.WellStructured`?
+-- -/
+-- theorem value_symbolize?_ok_same
+--   {Γ : TypeEnv} {entities : Entities} {v : Value} {ty : CedarType}
+--   (hwf : Γ.WellFormed)
+--   (hwf_ty : ty.WellFormed Γ)
+--   (hwf_v : v.WellFormed entities)
+--   (hwt : InstanceOfType Γ v ty) :
+--   ∃ t,
+--     v.symbolize? ty = .some t ∧
+--     v ∼ t
+-- := by
+--   sorry
+--   -- cases hwt with
+--   -- | instance_of_bool
+--   -- | instance_of_string
+--   -- | instance_of_entity
+--   -- | instance_of_ext
+--   -- | instance_of_int =>
+--   --   simp [
+--   --     Value.symbolize?, Prim.symbolize,
+--   --     Same.same, SameValues,
+--   --     Term.value?, TermPrim.value?, BitVec.int64?,
+--   --   ]
+--   -- | instance_of_set s sty hwt =>
+--   --   cases hwf_ty with | set_wf hwf_sty =>
+--   --   cases hwf_v with | set_wf hwf_v hwf_s =>
+--   --   -- `symbolize?` on elements should succeed
+--   --   have ⟨ts, hts⟩ :
+--   --     ∃ ts,
+--   --       s.toList.mapM (fun v => v.symbolize? sty) = .some ts
+--   --   := by
+--   --     apply List.all_some_implies_mapM_some
+--   --     intros x hmem_x
+--   --     have := hwt x hmem_x
+--   --     have ⟨t, ht, _⟩ := value_symbolize?_same hwf hwf_sty (hwf_v x hmem_x) this
+--   --     exists t
+--   --   -- `value? ∘ symbolize?` should succeed on elements
+--   --   have ⟨vs, hvs⟩ :
+--   --     ∃ vs,
+--   --       (Set.make ts).1.mapM (λ t => t.value?) = .some vs
+--   --   := by
+--   --     apply List.all_some_implies_mapM_some
+--   --     intros t hmem_t
+--   --     have := (Set.make_mem _ _).mpr hmem_t
+--   --     have hts := List.mapM_some_implies_all_from_some hts
+--   --     have ⟨x, hmem_x, hsym_x⟩ := hts t this
+--   --     have hwt_x := hwt x hmem_x
+--   --     have ⟨y, hy, hsame_y⟩ := value_symbolize?_same hwf hwf_sty (hwf_v x hmem_x) hwt_x
+--   --     simp only [hsym_x, Option.some.injEq] at hy
+--   --     exists x
+--   --     simp only [←hy] at hsame_y
+--   --     exact hsame_y
+--   --   simp only [
+--   --     Value.symbolize?,
+--   --     List.mapM₁_eq_mapM (λ v => v.symbolize? sty) s.toList,
+--   --   ]
+--   --   simp only [
+--   --     hts, Option.bind_some_fun,
+--   --     Option.some.injEq, exists_eq_left',
+--   --     Same.same, SameValues,
+--   --   ]
+--   --   unfold Term.value?
+--   --   simp only [
+--   --     List.mapM₁_eq_mapM ?_ (Set.make ts).1,
+--   --   ]
+--   --   simp only [hvs, Option.bind_some_fun, Option.some.injEq, Value.set.injEq]
+--   --   -- Prove that the sets of values before and after `value? ∘ symbolize?` are equal
+--   --   apply (Set.subset_iff_eq (Set.make_wf _) hwf_s).mp
+--   --   constructor
+--   --   · apply Set.subset_def.mpr
+--   --     intros new_v hmem_new_v
+--   --     have hmem_new_v := (Set.make_mem _ _).mpr hmem_new_v
+--   --     have ⟨x, hmem_x, hx_value?⟩ := List.mapM_some_implies_all_from_some hvs new_v hmem_new_v
+--   --     have hmem_x := (Set.make_mem _ _).mpr hmem_x
+--   --     have ⟨old_v, hmem_old_v, hold_v_symbolic?⟩ := List.mapM_some_implies_all_from_some hts x hmem_x
+
+--   --     sorry
+--   --   · sorry
+--   -- | instance_of_record rec =>
+--   --   sorry
 
 theorem env_symbolize?_same_request
   {Γ : TypeEnv} {env : Env}
+  (hwf_env : env.StronglyWellFormed)
   (hinst : InstanceOfWellFormedEnvironment env.request env.entities Γ) :
   env.request ∼ ((SymEnv.ofEnv Γ).interpret (env.symbolize? Γ)).request
 := by
@@ -90,13 +610,17 @@ theorem env_symbolize?_same_request
     have hwt_ctx : InstanceOfType Γ env.request.context (.record Γ.reqty.context) := by
       have ⟨_, ⟨_, _, _, h⟩, _⟩ := hinst
       exact h
-    have ⟨sym_ctx, hsym_ctx, hsame_sym_ctx⟩ := value_symbolize?_same hwf hwf_ctx_ty hwt_ctx
+    have hwf_ctx : (Value.record env.request.context).WellFormed env.entities := by
+      have ⟨⟨_, _, _, h⟩, _⟩ := hwf_env
+      exact h
+    have ⟨sym_ctx, hsym_ctx, hsame_sym_ctx⟩ := value?_symbolize?_id hwf hwf_ctx_ty hwf_ctx hwt_ctx
     simp only [Value.symbolize?, Option.bind_eq_bind] at hsym_ctx
     simp only [Option.bind_eq_bind, hsym_ctx]
     exact hsame_sym_ctx
 
 theorem env_symbolize?_same_entities
   {Γ : TypeEnv} {env : Env}
+  (hwf_env : env.StronglyWellFormed)
   (hinst : InstanceOfWellFormedEnvironment env.request env.entities Γ) :
   env.entities ∼ ((SymEnv.ofEnv Γ).interpret (env.symbolize? Γ)).entities
 := by
@@ -104,15 +628,17 @@ theorem env_symbolize?_same_entities
 
 theorem env_symbolize?_same
   {Γ : TypeEnv} {env : Env}
+  (hwf_env : env.StronglyWellFormed)
   (hinst : InstanceOfWellFormedEnvironment env.request env.entities Γ) :
   env ∼ (SymEnv.ofEnv Γ).interpret (env.symbolize? Γ)
 := by
   constructor
-  · exact env_symbolize?_same_request hinst
-  · exact env_symbolize?_same_entities hinst
+  · exact env_symbolize?_same_request hwf_env hinst
+  · exact env_symbolize?_same_entities hwf_env hinst
 
 theorem ofEnv_soundness
   {Γ : TypeEnv} {env : Env}
+  (hwf_env : env.StronglyWellFormed)
   (hinst : InstanceOfWellFormedEnvironment env.request env.entities Γ) :
   env ∈ᵢ SymEnv.ofEnv Γ
 := by
@@ -120,6 +646,6 @@ theorem ofEnv_soundness
   exists env.symbolize? Γ
   constructor
   · sorry
-  . exact env_symbolize?_same hinst
+  . exact env_symbolize?_same hwf_env hinst
 
 end Cedar.Thm
